Logic/Modal/Kripke/Geach.lean
@@ -265,7 +265,7 @@ lemma geachConfluent_CanonicalFrame (h : 𝗴𝗲(t) ⊆ Ax) : GeachConfluent t 
         (show 𝝂Ax ⊢! □^[t.n]⋀Δ ➝ □^[t.n](∼⋀Γ) by exact imply_multibox_distribute'! $ contra₁'! $ imp_trans''! (and_imply_iff_imply_imply'!.mp hC) (and₂'! neg_equiv!))
         (show 𝝂Ax ⊢! □^[t.n](∼⋀Γ) ➝ (◇^[t.n]⋀Γ) ➝ ⊥ by exact imp_trans''! (contra₁'! $ and₁'! $ multidia_duality!) (and₁'! neg_equiv!));
     }
-    have : 𝝂Ax ⊬! □^[t.n]⋀Δ ⋏ ◇^[t.n]⋀Γ ➝ ⊥ := by simpa using (def_consistent.mp Ω₃.consistent) (Γ := [□^[t.n]⋀Δ, ◇^[t.n]⋀Γ]) (by simp_all)
+    have : 𝝂Ax ⊬ □^[t.n]⋀Δ ⋏ ◇^[t.n]⋀Γ ➝ ⊥ := by simpa using (def_consistent.mp Ω₃.consistent) (Γ := [□^[t.n]⋀Δ, ◇^[t.n]⋀Γ]) (by simp_all)
 
     contradiction;
 
